coq/Impl.v
@@ -26,27 +26,35 @@ Module Type IMPL.
 
   Parameter intersect : pat -> pat -> pat.
   Parameter is_overlapped : pat -> pat -> bool.
-  Parameter is_match : pkt -> pat -> bool.
-  Parameter exact_match : pkt -> pat.
+  Parameter is_match : pkt -> port -> pat -> bool.
+  Parameter exact_match : pkt -> port -> pat.
 
-  Axiom no_match_subset_l : forall pkt m1 m2,
-    is_match pkt m1 = false ->
-    is_match pkt (intersect m1 m2) = false.
+  Section Axioms.
+
+    Variable k : pkt.
+    Variable m1 m2 m m': pat.
+    Variable n : port.
+
+    Axiom no_match_subset_l : 
+      is_match k n m1 = false ->
+      is_match k n (intersect m1 m2) = false.
+
+    Axiom no_match_subset_r :
+      is_match k n m1 = false ->
+      is_match k n (intersect m2 m1) = false.
   
-  Axiom no_match_subset_r : forall pkt m1 m2,
-    is_match pkt m2 = false ->
-    is_match pkt (intersect m1 m2) = false.
+    Axiom pkt_match_intersect :
+      is_match k n m = true -> 
+      is_match k n m' = true ->
+      is_match k n (intersect m m') = true.
+
+    Axiom packet_split : 
+      is_overlapped m1 m2 = false ->
+      is_match k n m1 = true  ->
+      is_match k n m2 = false.
+
+  End Axioms.
   
-  Axiom pkt_match_intersect : forall pkt m m',
-    is_match pkt m = true -> 
-    is_match pkt m' = true ->
-    is_match pkt (intersect m m') = true.
-
-  Axiom packet_split : forall pkt m1 m2,
-    is_overlapped m1 m2 = false ->
-    is_match pkt m1 = true  ->
-    is_match pkt m2 = false.
-
   Hint Rewrite pkt_eq_dec pat_eq_dec packet_split
     no_match_subset_l no_match_subset_r : packet.
 
